Logic/Propositional/Superintuitionistic/Kripke/Semantics.lean
@@ -83,60 +83,85 @@ variable
 
 @[simp] protected lemma iff_models : M ⊧ p ↔ Formula.Kripke.ValidOnModel M p := iff_of_eq rfl
 
-@[simp] protected lemma verum : M ⊧ ⊤ := by simp_all [ValidOnModel];
+protected lemma verum : M ⊧ ⊤ := by simp_all [ValidOnModel];
 
-@[simp] protected lemma and₁ : M ⊧ p ⋏ q ⟶ p := by simp_all [ValidOnModel, Satisfies];
+protected lemma and₁ : M ⊧ p ⋏ q ⟶ p := by simp_all [ValidOnModel, Satisfies];
 
-@[simp] protected lemma and₂ : M ⊧ p ⋏ q ⟶ q := by simp_all [ValidOnModel, Satisfies];
+protected lemma and₂ : M ⊧ p ⋏ q ⟶ q := by simp_all [ValidOnModel, Satisfies];
 
-@[simp] protected lemma and₃ : M ⊧ p ⟶ q ⟶ p ⋏ q := by
+protected lemma and₃ : M ⊧ p ⟶ q ⟶ p ⋏ q := by
   intro x y _ hp z Ryz hq;
   replace hp : Satisfies M z p := formula_hereditary atom_hereditary F_trans Ryz hp;
   exact ⟨hp, hq⟩;
 
-@[simp] protected lemma or₁ : M ⊧ p ⟶ p ⋎ q := by simp_all [ValidOnModel, Satisfies];
+protected lemma or₁ : M ⊧ p ⟶ p ⋎ q := by simp_all [ValidOnModel, Satisfies];
 
-@[simp] protected lemma or₂ : M ⊧ q ⟶ p ⋎ q := by simp_all [ValidOnModel, Satisfies];
+protected lemma or₂ : M ⊧ q ⟶ p ⋎ q := by simp_all [ValidOnModel, Satisfies];
 
-@[simp] protected lemma or₃ : M ⊧ (p ⟶ r) ⟶ (q ⟶ r) ⟶ (p ⋎ q ⟶ r) := by
+protected lemma or₃ : M ⊧ (p ⟶ r) ⟶ (q ⟶ r) ⟶ (p ⋎ q ⟶ r) := by
   simp_all only [ValidOnModel.iff_models, ValidOnModel, Satisfies.iff_models, Satisfies.imp_def, Satisfies.or_def];
   intro w₁ w₂ _ hpr w₃ hw₂₃ hqr w₄ hw₃₄ hpq;
   cases hpq with
   | inl hp => exact hpr (F_trans hw₂₃ hw₃₄) hp;
   | inr hq => exact hqr hw₃₄ hq;
 
-@[simp] protected lemma imply₁ : M ⊧ p ⟶ q ⟶ p := by
+protected lemma imply₁ : M ⊧ p ⟶ q ⟶ p := by
   intro x y _ hp z Ryz _;
   exact formula_hereditary atom_hereditary F_trans Ryz hp;
 
-@[simp] protected lemma imply₂ : M ⊧ (p ⟶ q ⟶ r) ⟶ (p ⟶ q) ⟶ p ⟶ r := by
+protected lemma imply₂ : M ⊧ (p ⟶ q ⟶ r) ⟶ (p ⟶ q) ⟶ p ⟶ r := by
   intro x y _ hpqr z Ryz hpq w Rzw hp;
   have Ryw := F_trans Ryz Rzw;
   have Rww := F_refl w;
   exact hpqr Ryw hp Rww (hpq Rzw hp);
 
-@[simp] protected lemma mdp (hpq : M ⊧ p ⟶ q) (hp : M ⊧ p) : M ⊧ q := by
+protected lemma mdp (hpq : M ⊧ p ⟶ q) (hp : M ⊧ p) : M ⊧ q := by
   intro w;
   exact hpq w (F_refl w) $ hp w;
 
-@[simp] protected lemma efq : M ⊧ Axioms.EFQ p := by simp [ValidOnModel, Satisfies];
+protected lemma efq : M ⊧ Axioms.EFQ p := by simp [ValidOnModel, Satisfies];
 
-@[simp] protected lemma neg_equiv : M ⊧ Axioms.NegEquiv p := by
+protected lemma neg_equiv : M ⊧ Axioms.NegEquiv p := by
   simp_all [ValidOnModel, Axioms.NegEquiv];
   intro w;
   constructor;
   . intro x _ h y rxy hyp; exact h rxy hyp;
   . intro x _ h y rxy; exact h rxy;
 
-@[simp] protected lemma lem (hExt : Extensive M.Frame.Rel) : M ⊧ Axioms.LEM p := by
+protected lemma lem (F_ext : Extensive M.Frame.Rel) : M ⊧ Axioms.LEM p := by
   simp_all [ValidOnModel];
   intro w;
   by_cases h : w ⊧ p
   . left; assumption;
   . right;
     intro w' hww';
-    rw [←(hExt hww')];
+    rw [←(F_ext hww')];
     assumption;
+
+protected lemma dum : Connected M.Frame.Rel → M ⊧ Axioms.GD p q := by
+  simp [ValidOnModel, Satisfies, Connected];
+  contrapose; push_neg;
+  rintro ⟨x, ⟨y, Rxy, hyp, nhyq⟩, ⟨z, Ryz, hzq, nhyp⟩⟩;
+  use x, y, z;
+  refine ⟨Rxy, Ryz, ?_, ?_⟩;
+  . by_contra Ryz;
+    have := formula_hereditary atom_hereditary F_trans Ryz hyp;
+    contradiction;
+  . by_contra Rzy;
+    have := formula_hereditary atom_hereditary F_trans Rzy hzq;
+    contradiction;
+
+protected lemma wlem : Confluent M.Frame.Rel → M ⊧ Axioms.WeakLEM p := by
+  simp [ValidOnModel, Satisfies, Confluent];
+  contrapose; push_neg;
+  rintro ⟨x, ⟨y, Rxy, hyp⟩, ⟨z, Rxz, hz⟩⟩;
+  use x, y, z;
+  refine ⟨Rxy, Rxz, ?_⟩;
+  rintro w Ryw;
+  by_contra Rzw;
+  have := formula_hereditary atom_hereditary F_trans Ryw hyp;
+  have := hz w Rzw;
+  contradiction;
 
 end ValidOnModel
 
@@ -155,31 +180,35 @@ variable {F : Frame.Dep α} {p q r : Formula α}
          (F_trans : Transitive F)
          (F_refl : Reflexive F)
 
-@[simp] protected lemma verum : F ⊧ ⊤ := fun _ => ValidOnModel.verum
+protected lemma verum : F ⊧ ⊤ := fun _ => ValidOnModel.verum
 
-@[simp] protected lemma and₁ : F ⊧ p ⋏ q ⟶ p := fun _ => ValidOnModel.and₁
+protected lemma and₁ : F ⊧ p ⋏ q ⟶ p := fun _ => ValidOnModel.and₁
 
-@[simp] protected lemma and₂ : F ⊧ p ⋏ q ⟶ q := fun _ => ValidOnModel.and₂
+protected lemma and₂ : F ⊧ p ⋏ q ⟶ q := fun _ => ValidOnModel.and₂
 
-@[simp] protected lemma and₃ : F ⊧ p ⟶ q ⟶ p ⋏ q := fun hV => ValidOnModel.and₃ hV F_trans
+protected lemma and₃ : F ⊧ p ⟶ q ⟶ p ⋏ q := fun hV => ValidOnModel.and₃ hV F_trans
 
-@[simp] protected lemma or₁ : F ⊧ p ⟶ p ⋎ q := fun _ => ValidOnModel.or₁
+protected lemma or₁ : F ⊧ p ⟶ p ⋎ q := fun _ => ValidOnModel.or₁
 
-@[simp] protected lemma or₂ : F ⊧ q ⟶ p ⋎ q := fun _ => ValidOnModel.or₂
+protected lemma or₂ : F ⊧ q ⟶ p ⋎ q := fun _ => ValidOnModel.or₂
 
-@[simp] protected lemma or₃ : F ⊧ (p ⟶ r) ⟶ (q ⟶ r) ⟶ (p ⋎ q ⟶ r) := fun _ => ValidOnModel.or₃ F_trans
+protected lemma or₃ : F ⊧ (p ⟶ r) ⟶ (q ⟶ r) ⟶ (p ⋎ q ⟶ r) := fun _ => ValidOnModel.or₃ F_trans
 
-@[simp] protected lemma imply₁ : F ⊧ p ⟶ q ⟶ p := fun hV => ValidOnModel.imply₁ hV F_trans
+protected lemma imply₁ : F ⊧ p ⟶ q ⟶ p := fun hV => ValidOnModel.imply₁ hV F_trans
 
-@[simp] protected lemma imply₂ : F ⊧ (p ⟶ q ⟶ r) ⟶ (p ⟶ q) ⟶ p ⟶ r := fun _ => ValidOnModel.imply₂ F_trans F_refl
+protected lemma imply₂ : F ⊧ (p ⟶ q ⟶ r) ⟶ (p ⟶ q) ⟶ p ⟶ r := fun _ => ValidOnModel.imply₂ F_trans F_refl
 
-@[simp] protected lemma mdp (hpq : F ⊧ p ⟶ q) (hp : F ⊧ p) : F ⊧ q := fun hV => ValidOnModel.mdp F_refl (hpq hV) (hp hV)
+protected lemma mdp (hpq : F ⊧ p ⟶ q) (hp : F ⊧ p) : F ⊧ q := fun hV => ValidOnModel.mdp F_refl (hpq hV) (hp hV)
 
-@[simp] protected lemma efq : F ⊧ Axioms.EFQ p := fun _ => ValidOnModel.efq
+protected lemma efq : F ⊧ Axioms.EFQ p := fun _ => ValidOnModel.efq
 
-@[simp] protected lemma neg_equiv : F ⊧ Axioms.NegEquiv p := fun _ => ValidOnModel.neg_equiv
+protected lemma neg_equiv : F ⊧ Axioms.NegEquiv p := fun _ => ValidOnModel.neg_equiv
 
-@[simp] protected lemma lem (hExt : Extensive F.Rel) : F ⊧ Axioms.LEM p := fun _ => ValidOnModel.lem hExt
+protected lemma lem (hExt : Extensive F.Rel) : F ⊧ Axioms.LEM p := fun _ => ValidOnModel.lem hExt
+
+protected lemma dum (F_conn : Connected F.Rel) : F ⊧ Axioms.GD p q := fun hV => ValidOnModel.dum hV F_trans F_conn
+
+protected lemma wlem (F_conf : Confluent F.Rel) : F ⊧ Axioms.WeakLEM p := fun hV => ValidOnModel.wlem hV F_trans F_conf
 
 instance : Semantics.Bot (Frame.Dep α) where
   realize_bot _ := by
@@ -247,7 +276,7 @@ end Soundness
 
 variable {α : Type u}
 
-instance Int_Characteraizable : 𝔽(𝐈𝐧𝐭 of α).Characteraizable (λ F => Transitive F ∧ Reflexive F) where
+instance Int_Characteraizable : 𝔽(𝐈𝐧𝐭 of α).Characteraizable (λ F => Reflexive F ∧ Transitive F) where
   characterize := by
     simp [System.theory];
     intro F hTrans hRefl p hp;
@@ -272,12 +301,12 @@ instance Int_Characteraizable : 𝔽(𝐈𝐧𝐭 of α).Characteraizable (λ F 
     use { World := PUnit, Rel := λ _ _ => True };
     simp [Transitive, Reflexive];
 
-instance : Sound 𝐈𝐧𝐭 (TransitiveReflexiveFrameClass#α) := inferInstance
+instance : Sound 𝐈𝐧𝐭 (ReflexiveTransitiveFrameClass#α) := inferInstance
 
 instance : System.Consistent (𝐈𝐧𝐭 : DeductionParameter α) := inferInstance
 
 
-instance Cl_Characteraizable : 𝔽(𝐂𝐥 of α).Characteraizable (λ F => Transitive F ∧ Reflexive F ∧ Extensive F) where
+instance Cl_Characteraizable : 𝔽(𝐂𝐥 of α).Characteraizable (λ F => Reflexive F ∧ Transitive F ∧ Extensive F) where
   characterize := by
     simp [System.theory];
     intro F hTrans hRefl hExt p hp;
@@ -303,9 +332,74 @@ instance Cl_Characteraizable : 𝔽(𝐂𝐥 of α).Characteraizable (λ F => Tr
     use { World := PUnit, Rel := λ _ _ => True };
     simp [Transitive, Reflexive, Extensive];
 
-instance : Sound 𝐂𝐥 (TransitiveReflexiveExtensiveFrameClass#α) := inferInstance
+instance : Sound 𝐂𝐥 (ReflexiveTransitiveExtensiveFrameClass#α) := inferInstance
 
 instance : System.Consistent (𝐂𝐥 : DeductionParameter α) := inferInstance
+
+
+
+instance KC_Characteraizable : 𝔽(𝐊𝐂 of α).Characteraizable (λ F => Reflexive F ∧ Transitive F ∧ Confluent F) where
+  characterize := by
+    rintro F ⟨F_trans, F_refl, F_confl⟩;
+    simp [System.theory];
+    intro p hp;
+    induction hp using Deduction.rec! with
+    | verum => apply ValidOnFrame.verum;
+    | imply₁ => apply ValidOnFrame.imply₁; simpa;
+    | imply₂ => apply ValidOnFrame.imply₂; simpa; simpa;
+    | and₁ => apply ValidOnFrame.and₁;
+    | and₂ => apply ValidOnFrame.and₂;
+    | and₃ => apply ValidOnFrame.and₃; simpa;
+    | or₁ => apply ValidOnFrame.or₁;
+    | or₂ => apply ValidOnFrame.or₂;
+    | or₃ => apply ValidOnFrame.or₃; simpa;
+    | neg_equiv => apply ValidOnFrame.neg_equiv;
+    | mdp ihpq ihp =>
+      apply ValidOnFrame.mdp;
+      repeat simpa;
+    | eaxm h =>
+      rcases h with (⟨_, rfl⟩ | ⟨_, _, rfl⟩);
+      . apply ValidOnFrame.efq;
+      . apply ValidOnFrame.wlem; simpa; simpa;
+  nonempty := by
+    use { World := PUnit, Rel := λ _ _ => True };
+    simp [Transitive, Reflexive, Confluent];
+
+instance : Sound 𝐊𝐂 (ReflexiveTransitiveConfluentFrameClass#α) := inferInstance
+
+instance : System.Consistent (𝐊𝐂 : DeductionParameter α) := inferInstance
+
+
+instance LC_Characteraizable : 𝔽(𝐋𝐂 of α).Characteraizable (λ F => Reflexive F ∧ Transitive F ∧ Connected F) where
+  characterize := by
+    rintro F ⟨F_trans, F_refl, F_conn⟩;
+    simp [System.theory];
+    intro p hp;
+    induction hp using Deduction.rec! with
+    | verum => apply ValidOnFrame.verum;
+    | imply₁ => apply ValidOnFrame.imply₁; simpa;
+    | imply₂ => apply ValidOnFrame.imply₂; simpa; simpa;
+    | and₁ => apply ValidOnFrame.and₁;
+    | and₂ => apply ValidOnFrame.and₂;
+    | and₃ => apply ValidOnFrame.and₃; simpa;
+    | or₁ => apply ValidOnFrame.or₁;
+    | or₂ => apply ValidOnFrame.or₂;
+    | or₃ => apply ValidOnFrame.or₃; simpa;
+    | neg_equiv => apply ValidOnFrame.neg_equiv;
+    | mdp ihpq ihp =>
+      apply ValidOnFrame.mdp;
+      repeat simpa;
+    | eaxm h =>
+      rcases h with (⟨_, rfl⟩ | ⟨_, _, rfl⟩);
+      . apply ValidOnFrame.efq;
+      . apply ValidOnFrame.dum; simpa; simpa;
+  nonempty := by
+    use { World := PUnit, Rel := λ _ _ => True };
+    simp [Transitive, Reflexive, Connected];
+
+instance : Sound 𝐋𝐂 (ReflexiveTransitiveConnectedFrameClass#α) := inferInstance
+
+instance : System.Consistent (𝐋𝐂 : DeductionParameter α) := inferInstance
 
 end Kripke
 
