Logic/Vorspiel/BinaryRelations.lean
@@ -11,7 +11,7 @@ def Euclidean := ∀ ⦃w₁ w₂ w₃⦄, w₁ ≺ w₂ → w₁ ≺ w₃ → w
 
 def Serial := ∀ w₁, ∃ w₂, w₁ ≺ w₂
 
-def Confluent := ∀ ⦃w₁ w₂ w₃⦄, ((w₁ ≺ w₂ ∧ w₁ ≺ w₃) → ∃ w₄, w₂ ≺ w₄ ∧ w₃ ≺ w₄)
+def Confluent := ∀ ⦃x y z⦄, ((x ≺ y ∧ x ≺ z) → ∃ w, (y ≺ w ∧ z ≺ w))
 
 def Dense := ∀ ⦃w₁ w₂⦄, w₁ ≺ w₂ → ∃w₃, w₁ ≺ w₃ ∧ w₃ ≺ w₂
 
